new/golang/defn/dynamic_mem.v
@@ -1,0 +1,55 @@
+From Perennial.goose_lang Require Import lang notation.
+From New.golang.defn Require Import assume list dynamic_typing.
+From New.golang.defn Require Export typing.
+From Perennial Require Import base.
+
+(* note: same names as mem.v, use only one of the two *)
+Section defn.
+Context `{ffi_syntax}.
+
+Definition load_ty_def: val :=
+  rec: "go" "t" "l" :=
+    type.Match "t"
+      (λ: <>, !"l")
+      (λ: "n" "t",
+        let: "size" := type.go_type_size "t" in
+        (rec: "go_arr" "n" "l" :=
+           let: "l_new" := "l" +ₗ "size" in
+           if: "n" = #(W64 0) then #()
+           else ("go" "t" "l", "go_arr" ("n" - #(W64 1)) "l_new")
+        ) "n" "l")
+      (λ: "decls",
+        (rec: "go_struct" "decls" "l" :=
+           list.Match "decls"
+                      (λ: <>, #())
+                      (λ: "hd" "decls", let: ("f", "t") := "hd" in
+                          ("go" "t" "l", "go_struct" "decls" ("l" +ₗ type.go_type_size "t")))
+        ) "decls" "l")
+      .
+Program Definition load_ty := sealed @load_ty_def.
+Definition load_ty_unseal : @load_ty = _ := seal_eq _.
+
+Definition store_ty_def: val :=
+  rec: "go" "t" "l" "v" :=
+    type.Match "t"
+      (λ: <>, "l" <- "v")
+      (λ: "n" "t",
+        let: "size" := type.go_type_size "t" in
+        (rec: "go_arr" "n" "l" "v" :=
+           let: "l_new" := "l" +ₗ "size" in
+           if: "n" = #(W64 0) then #()
+           else "go" "t" "l" (Fst "v");; "go_arr" ("n" - #(W64 1)) "l_new" (Snd "v")
+        ) "n" "l" "v")
+      (λ: "decls",
+        (rec: "go_struct" "decls" "l" "v" :=
+           list.Match "decls"
+                      (λ: <>, #())
+                      (λ: "hd" "decls", let: ("f", "t") := "hd" in
+                          "go" "t" "l" (Fst "v");;
+                          "go_struct" "decls" ("l" +ₗ type.go_type_size "t") (Snd "v"))
+        ) "decls" "l" "v")
+      .
+Program Definition store_ty := sealed @store_ty_def.
+Definition store_ty_unseal : @store_ty = _ := seal_eq _.
+
+End defn.
