new/golang/theory.v
@@ -1,5 +1,7 @@
 From Perennial.goose_lang Require Export lang.
 From New.golang Require Export defn.
+(* NOTE: unused for now but still should be compiled *)
+From New.golang.theory Require dynamic_mem.
 From New.golang.theory Require Export exception list typing dynamic_typing loop struct
   mem slice map interface defer typing builtin primitive chan pkg auto globals.
 
