new/golang/theory/dynamic_typing.v
@@ -1,4 +1,3 @@
-From Coq Require Import Logic.FunctionalExtensionality.
 From Coq Require Import Program.Equality.
 From Ltac2 Require Import Ltac2.
 Set Default Proof Mode "Classic".
@@ -79,10 +78,10 @@ Qed.
 
 Lemma wp_type_size (t: go_type) stk E :
   {{{ True }}}
-    type.go_type_size_e #t @ stk; E
+    type.go_type_size #t @ stk; E
   {{{ RET (#(W64 (Z.of_nat (go_type_size t)))); £1 ∗ ⌜Z.of_nat (go_type_size t) < 2^64⌝ }}}.
 Proof.
-  rewrite type.go_type_size_e_unseal.
+  rewrite type.go_type_size_unseal.
   rewrite go_type_size_unseal.
 
   induction t using go_type_ind; iIntros (Φ) "_ HΦ"; wp_call_lc "Hlc";
@@ -120,154 +119,12 @@ Qed.
 (* note: not an instance to take advantage of overflow assumption *)
 Lemma wp_type_size_pure_wp (t: go_type) :
   PureWp True
-         (type.go_type_size_e #t)
+         (type.go_type_size #t)
          (#(W64 (Z.of_nat (go_type_size t)))).
 Proof.
   intros ?????; iIntros "Hwp".
   wp_apply wp_type_size. iIntros "[? %]".
   iApply ("Hwp" with "[$]").
 Qed.
-
-Context `{!IntoValTyped V t}.
-
-Lemma wp_load_ty l (v: V) q :
-  {{{ ▷ l ↦{q} v }}}
-    type.load_ty #t #l
-  {{{ RET #v; l ↦{q} v }}}.
-Proof.
-  (*
-  iIntros (Φ) ">Hl HΦ".
-  rewrite type.load_ty_unseal /=.
-  rewrite typed_pointsto_unseal /typed_pointsto_def.
-  pose proof (to_val_has_go_type v) as Hty.
-  generalize dependent (# v). clear dependent V.
-  intros v Hty.
-  rename l into l'.
-  iInduction Hty as [] "IH" forall (l' Φ) "HΦ".
-  all: try destruct i.
-  all: rewrite ?[in flatten_struct _]to_val_unseal /= /= ?loc_add_0 ?right_id; wp_pures.
-  all:
-    try solve [ wp_call; rewrite !to_val_unseal /=;
-                           iApply (wp_load with "[$]");
-                iIntros "!> H"; rewrite ?to_val_unseal /=; iApply "HΦ"; done
-      ].
-
-  {
-    wp_call.
-    replace n with (W64 (uint.nat n)) in * by word.
-    assert (Z.of_nat (uint.nat n) < 2^64) by word.
-    generalize dependent (uint.nat n); clear n; intros n Hty Hbound.
-    clear Hty.
-    iInduction n as [|n] "IHn" forall (l' a Φ).
-    - admit.
-    - rewrite (bool_decide_eq_false_2 (W64 (S n) = W64 0)); [ wp_pures | word ].
-      destruct a as [|t' a']; simpl in *; [ word | ].
-      iDestruct (big_sepL_app with "Hl") as "[Hl1 Hl2]".
-      wp_apply ("IH" with "[] [$Hl1]").
-      { naive_solver. }
-      iIntros "Hl1".
-      wp_pures.
-      replace (word.sub (W64 (S n)) (W64 1)) with (W64 n) by word.
-      wp_bind (If _ _ _).
-      rewrite Z.mul_1_l.
-      iApply "IHn".
-      iApply ("IH" $! _ _ (foldr PairV (#()) a') with "[] [] [Hl2]").
-      { iPureIntro. apply has_go_type_array.
-        - word.
-        - naive_solver. }
-      {
-        iPureIntro. rewrite app_length in Hlen.
-        apply has_go_type_len in H.
-  }
-   *)
-
-  rewrite type.load_ty_unseal /=.
-  rewrite typed_pointsto_unseal /typed_pointsto_def.
-  pose proof (to_val_has_go_type v) as Hty.
-  generalize dependent (# v). clear dependent V.
-  generalize dependent l.
-  induction t using go_type_ind;
-    iIntros (l v Hty Φ) ">Hl HΦ";
-    try solve [
-        wp_call;
-        inv Hty;
-        rewrite to_val_unseal /= ?loc_add_0 ?right_id;
-        iApply (wp_load with "[$Hl]");
-        iFrame
-      ].
-  - wp_call.
-    replace n with (W64 (uint.nat n)) in * by word.
-    assert (Z.of_nat (uint.nat n) < 2^64) by word.
-    generalize dependent (uint.nat n); clear n; intros n Hty Hbound.
-    wp_apply wp_type_size. iIntros "[_ %Hsz]". wp_pures.
-    iInduction n as [|n] "IH" forall (l v Hty Φ).
-    + rewrite bool_decide_eq_true_2; [ wp_pures | word ].
-      inv Hty.
-      assert (a = []) by (destruct a; naive_solver); subst; simpl.
-      rewrite to_val_unseal /=.
-      iApply "HΦ". iFrame.
-    + rewrite (bool_decide_eq_false_2 (W64 (S n) = W64 0)); [ wp_pures | word ].
-      assert (length (flatten_struct v) = (S n * go_type_size g)%nat) as Hlen.
-      {
-        apply has_go_type_len in Hty.
-        rewrite Hty.
-        rewrite go_type_size_unseal /=.
-        rewrite -go_type_size_unseal.
-        replace (uint.nat (W64 (S n))) with (S n) by word.
-        reflexivity.
-      }
-      pose proof Hty as Hty'.
-      inv Hty.
-      destruct a as [|t' a']; simpl in *; [ word | ].
-      rewrite length_app in Hlen.
-      assert (has_go_type t' g) as Ht' by naive_solver.
-      pose proof Ht' as Hlen'. apply has_go_type_len in Hlen'.
-      rewrite Hlen' in Hlen.
-      iDestruct (big_sepL_app with "Hl") as "[Hl1 Hl2]".
-      wp_apply (IHg with "[$Hl1]").
-      { auto. }
-      iIntros "Hl1".
-      wp_pures.
-      replace (word.sub (W64 (S n)) (W64 1)) with (W64 n) by word.
-      wp_bind (If _ _ _).
-      rewrite Z.mul_1_l.
-      iApply ("IH" $! _ _ (foldr PairV (#()) a') with "[] [Hl2]").
-      { iPureIntro. apply has_go_type_array.
-        - word.
-        - naive_solver. }
-      { rewrite Hlen'.
-        iApply (big_sepL_impl with "Hl2").
-        iIntros "!>" (???) "H".
-        iExactEq "H".
-        rewrite loc_add_assoc.
-        repeat (f_equal; try word). }
-      iIntros "Hl2".
-      wp_pures.
-      iApply "HΦ".
-      rewrite big_sepL_app.
-      rewrite Hlen'.
-      iFrame "Hl1".
-      iApply (big_sepL_impl with "Hl2").
-      iIntros "!>" (???) "H".
-      iExactEq "H".
-      rewrite loc_add_assoc.
-      repeat (f_equal; try word).
-  - inv Hty.
-    wp_call.
-    destruct i;
-      rewrite to_val_unseal /= ?loc_add_0 ?right_id;
-      iApply (wp_load with "[$Hl]");
-      iFrame.
-  - (* structT *)
-    wp_call.
-    admit.
-Admitted.
-
-Lemma wp_store_ty l (v0 v: V) :
-  {{{ ▷l ↦ v0 }}}
-    type.store_ty #t #l #v
-  {{{ RET #(); l ↦ v }}}.
-Proof.
-Admitted.
 
 End goose_lang.
